finish most of FmajorComp.I_sim

src/FmajorComp.v
@@ -1,6 +1,9 @@
 Require Import compcert.lib.Integers.
+Require Import compcert.lib.Maps.
 Require Import compcert.lib.Coqlib.
 Require Import compcert.common.AST.
+Require Import compcert.common.Events.
+Require Import compcert.common.Globalenvs.
 
 Require Import StructTact.Assoc.
 
@@ -18,6 +21,9 @@ Close Scope Z_scope.
 
 Module A := FlatIntTag.
 Module B := Fmajor.
+
+Add Printing Constructor A.frame.
+Add Printing Constructor B.function.
 
 
 Fixpoint count_up' acc n :=
@@ -106,7 +112,8 @@ Definition build_id_list (cu : list (A.stmt * A.expr) * list metadata) :
 Section compile.
 Open Scope option_monad.
 
-Variable M : list (id_key * ident).
+Definition id_map := list (id_key * ident).
+Variable M : id_map.
 Let get_id := id_key_assoc M.
 
 Definition compile_expr :=
@@ -183,10 +190,571 @@ Definition compile_func (f : A.stmt * A.expr) : option B.function :=
 
 End compile.
 
+Ltac refold_compile M :=
+    fold (compile_expr M) in *;
+    fold (compile_expr_list M) in *;
+    fold (compile_list M) in *.
+
+
+
+Section match_states.
+
+Variable M : id_map.
+
+Definition I_id k i := id_key_assoc M k = Some i.
+Hint Unfold I_id.
+
+Inductive I_expr : A.expr -> B.expr -> Prop :=
+| IArg : forall i,
+        I_id IkArg i ->
+        I_expr A.Arg (B.Var i)
+| ISelf : forall i,
+        I_id IkSelf i ->
+        I_expr A.Self (B.Var i)
+| IVar : forall i i',
+        I_id (IkVar i) i' ->
+        I_expr (A.Var i) (B.Var i')
+| IDeref : forall ae be off,
+        I_expr ae be ->
+        I_expr (A.Deref ae off) (B.Deref be off)
+.
+
+Inductive I_stmt : A.stmt -> B.stmt -> Prop :=
+| ISkip :
+        I_stmt A.Skip B.Sskip
+| ISeq : forall as1 as2 bs1 bs2,
+        I_stmt as1 bs1 ->
+        I_stmt as2 bs2 ->
+        I_stmt (A.Seq as1 as2) (B.Sseq bs1 bs2)
+| ICall : forall adst af aa bdst bf ba,
+        I_id (IkVar adst) bdst ->
+        I_expr af bf ->
+        I_expr aa ba ->
+        I_stmt (A.Call adst af aa) (B.Scall bdst bf ba)
+| IMkConstr : forall adst tag aargs bdst bargs,
+        I_id (IkVar adst) bdst ->
+        Forall2 I_expr aargs bargs ->
+        I_stmt (A.MkConstr adst tag aargs)
+               (B.SmakeConstr bdst tag bargs)
+| ISwitch : forall adst acases btargid bcases btarget,
+        I_id IkSwitchTarget btargid ->
+        I_expr A.Arg btarget ->
+        Forall2 (fun a b => fst a = fst b /\ I_stmt (snd a) (snd b)) acases bcases ->
+        I_stmt (A.Switch adst acases)
+               (B.Sswitch btargid bcases btarget)
+| IMkClose : forall adst afname afree bdst bfname bfree,
+        I_id (IkVar adst) bdst ->
+        I_id (IkFunc afname) bfname ->
+        Forall2 I_expr afree bfree ->
+        I_stmt (A.MkClose adst afname afree)
+               (B.SmakeClose bdst bfname bfree)
+| IAssign : forall adst ae bdst be,
+        I_id (IkVar adst) bdst ->
+        I_expr ae be ->
+        I_stmt (A.Assign adst ae)
+               (B.Sassign bdst be)
+.
+
+Inductive I_func : A.stmt * A.expr -> B.function -> Prop :=
+| IFunc : forall abody aret bself barg bbody bret,
+        I_id IkSelf bself ->
+        I_id IkArg barg ->
+        I_stmt abody bbody ->
+        I_expr aret bret ->
+        I_func (abody, aret)
+               (B.mkfunction [bself; barg] the_sig 0%Z (bbody, bret))
+.
+
+Inductive I_env : A.env -> B.genv -> Prop :=
+    (* TODO *)
+.
+
+Inductive I_value : value -> value -> Prop :=
+| IConstr : forall tag aargs bargs,
+        Forall2 I_value aargs bargs ->
+        I_value (Constr tag aargs) (Constr tag bargs)
+| IClose : forall afname afree bfname bfree,
+        I_id (IkFunc (pred (Pos.to_nat afname))) bfname ->
+        Forall2 I_value afree bfree ->
+        I_value (Close afname afree) (Close bfname bfree)
+.
+
+Inductive I_opt_value : value -> option value -> Prop :=
+| IOptValue : forall v1 v2,
+        I_value v1 v2 ->
+        I_opt_value v1 (Some v2).
+Hint Constructors I_opt_value.
+
+Inductive I_frame : A.frame -> B.env -> Prop :=
+| IFrame : forall aarg aself alocals barg_id bself_id blocals_ids benv,
+        I_id IkArg barg_id ->
+        I_id IkSelf bself_id ->
+        Forall2 (fun ai bi => I_id (IkVar ai) bi) (keys alocals) blocals_ids ->
+        I_opt_value aarg (benv ! barg_id) ->
+        I_opt_value aself (benv ! bself_id) ->
+        Forall2 (fun aentry bid => I_opt_value (snd aentry) (benv ! bid)) alocals blocals_ids ->
+        I_frame (A.Frame aarg aself alocals) benv
+.
+
+Inductive I_cont : A.cont -> B.cont -> Prop :=
+| IkSeq : forall acode ak bcode bk,
+        I_stmt acode bcode ->
+        I_cont ak bk ->
+        I_cont (A.Kseq acode ak)
+               (B.Kseq bcode bk)
+| IkSwitch : forall ak bk,
+        I_cont ak bk ->
+        I_cont (A.Kswitch ak)
+               (B.Kswitch bk)
+| IkReturn : forall aret ak bret bk,
+        I_expr aret bret ->
+        I_cont ak bk ->
+        B.is_call_cont bk ->
+        I_cont (A.Kreturn aret ak)
+               (B.Kreturn bret bk)
+| IkCall : forall adst af ak bdst be bk,
+        I_id (IkVar adst) bdst ->
+        I_frame af be ->
+        I_cont ak bk ->
+        be ! bdst = None ->
+        I_cont (A.Kcall adst af ak)
+               (B.Kcall bdst be bk)
+    (* TODO: handle stop states *)
+| IkStop : forall aret,
+        I_cont (A.Kstop aret)
+               (B.Kstop)
+.
+
+Inductive I : A.state -> B.state -> Prop :=
+| IRun : forall as_ af ak bs bk be,
+        I_stmt as_ bs ->
+        I_frame af be ->
+        I_cont ak bk ->
+        I (A.Run as_ af ak)
+          (B.State bs bk be)
+| IReturn : forall av ak bv bk,
+        I_value av bv ->
+        I_cont ak bk ->
+        I (A.Return av ak)
+          (B.Returnstate bv bk)
+.
+
+End match_states.
+Hint Resolve ISkip.
+Hint Unfold B.is_call_cont.
+
+
+
+Lemma compile_I_expr : forall M a b,
+    compile_expr M a = Some b ->
+    I_expr M a b.
+induction a;
+intros0 Hcomp; simpl in Hcomp; break_bind_option; inject_some; refold_compile M;
+try solve [constructor; eauto].
+Qed.
+
+Lemma compile_list_I_expr : forall M a b,
+    compile_expr_list M a = Some b ->
+    Forall2 (I_expr M) a b.
+induction a;
+intros0 Hcomp; simpl in Hcomp; break_bind_option; inject_some; refold_compile M;
+try solve [constructor; eauto using compile_I_expr].
+Qed.
+
+Lemma compile_I_stmt : forall M a b,
+    compile M a = Some b ->
+    I_stmt M a b.
+intro M.
+induction a using A.stmt_rect_mut with
+    (Pl := fun a => forall b,
+        compile_list M a = Some b ->
+        Forall2 (fun a b => fst a = fst b /\ I_stmt M (snd a) (snd b)) a b);
+intros0 Hcomp; simpl in Hcomp; break_bind_option; inject_some; refold_compile M;
+try solve [constructor; eauto using compile_I_expr, compile_list_I_expr].
+
+- (* Switch *)
+  constructor; eauto using compile_I_expr.
+  constructor. eauto.
+Qed.
+
+Lemma compile_I_func : forall M a b,
+    compile_func M a = Some b ->
+    I_func M a b.
+destruct a;
+intros0 Hcomp; simpl in Hcomp; break_bind_option; inject_some; refold_compile M;
+try solve [constructor; eauto using compile_I_expr, compile_I_stmt].
+Qed.
+
+
+
+Ltac i_ctor := intros; econstructor; simpl; eauto.
+Ltac i_lem H := intros; eapply H; simpl; eauto.
+
+Lemma set_I_opt_value : forall M v bf bid bid' v',
+    I_opt_value M v (bf ! bid) ->
+    bid' <> bid ->
+    I_opt_value M v ((PTree.set bid' v' bf) ! bid).
+intros0 II Hne.
+rewrite PTree.gso; eauto.
+Qed.
+
+Lemma set_I_frame : forall M af adst av bf bdst bv,
+    I_frame M af bf ->
+    I_id M (IkVar adst) bdst ->
+    I_value M av bv ->
+    bf ! bdst = None ->
+    I_frame M (A.set af adst av) (PTree.set bdst bv bf).
+intros0 II IIid IIval Hnone. invc II.
+unfold A.set. simpl. econstructor; eauto.
+- econstructor; eauto.
+- rewrite PTree.gso; eauto. repeat on >I_opt_value, invc. congruence.
+- rewrite PTree.gso; eauto. repeat on >I_opt_value, invc. congruence.
+- econstructor.
+    { rewrite PTree.gss. simpl. constructor. auto. }
+  unfold keys in *. rewrite <- Forall2_map_l in *.
+  list_magic_on (blocals_ids, (alocals, tt)).
+  destruct alocals_i as [ak av']. simpl in *.
+  rewrite PTree.gso; eauto. repeat on >I_opt_value, invc. congruence.
+Qed.
+Hint Resolve set_I_frame.
+
+Lemma set_switch_target_I_frame : forall M af bf bdst bv,
+    I_frame M af bf ->
+    I_id M IkSwitchTarget bdst ->
+    bf ! bdst = None ->
+    I_frame M af (PTree.set bdst bv bf).
+intros0 II IIid Hnone. invc II.
+unfold A.set. simpl. econstructor; eauto.
+- rewrite PTree.gso; eauto. repeat on >I_opt_value, invc. congruence.
+- rewrite PTree.gso; eauto. repeat on >I_opt_value, invc. congruence.
+- unfold keys in *. rewrite <- Forall2_map_l in *.
+  list_magic_on (blocals_ids, (alocals, tt)); cycle 1.
+    { (* automation broke :( *)
+      eapply nth_error_Forall2; eauto using Forall2_length.
+      intros. on _, eapply_; try eassumption.
+      - pattern x, y. eapply Forall2_nth_error; eauto.
+      - pattern x, y. eapply Forall2_nth_error; eauto.
+    }
+  destruct alocals_i as [ak av']. simpl in *.
+  rewrite PTree.gso; eauto. repeat on >I_opt_value, invc. congruence.
+Qed.
+Hint Resolve set_switch_target_I_frame.
+
+Hint Constructors I_value.
+
+(*
+Hint Constructors B.eval.
+
+Lemma local_sim : forall af bf l av,
+    I_frame af bf ->
+    A.local af l = Some av ->
+    exists bv,
+        B.local bf l = Some bv /\
+        I_value av bv.
+destruct af, bf.
+make_first locals. induction locals; intros0 II Alocal.
+- unfold A.local in *. simpl in *. discriminate.
+- destruct a as [k v].
+  invc II. on >Forall2, invc. destruct y. break_and. simpl in *.
+  unfold A.local, B.local in *. simpl in *.
+
+  destruct (eq_nat_dec l k).
+  + inject_some.
+    eexists. break_if; try congruence. eauto.
+  + break_if; try congruence. eauto.
+Qed.
+*)
+
+Lemma lookup_keys_nth_error : forall A xs k (x : A),
+    lookup xs k = Some x ->
+    exists n, nth_error (keys xs) n = Some k.
+intros.  eapply In_nth_error. eapply lookup_some_in_keys. eauto.
+Qed.
+
+Lemma lookup_some_in : forall A xs k (x : A),
+    lookup xs k = Some x ->
+    In (k, x) xs.
+first_induction xs; intros0 Hlook; simpl in *.
+- discriminate.
+- destruct a. break_if; inject_some; eauto.
+Qed.
+
+Lemma lookup_nth_error : forall A xs k (x : A),
+    lookup xs k = Some x ->
+    exists n, nth_error xs n = Some (k, x).
+intros.  eapply In_nth_error. eapply lookup_some_in. eauto.
+Qed.
+
+Lemma eval_sim : forall M af ae av bf be,
+    I_frame M af bf ->
+    I_expr M ae be ->
+    A.eval af ae av ->
+    exists bv,
+        B.eval_expr bf be bv /\
+        I_value M av bv.
+induction ae; intros0 IIframe IIexpr Aeval;
+inv IIframe; invc Aeval; invc IIexpr.
+
+- repeat on >I_opt_value, invc.
+  eexists; split; eauto. constructor. congruence.
+
+- repeat on >I_opt_value, invc.
+  eexists; split; eauto. constructor. congruence.
+
+- fwd eapply lookup_nth_error as HH; eauto. simpl in *. destruct HH as [n ?].
+  fwd eapply map_nth_error with (f := fst) (l := alocals); eauto.
+    simpl in *. change (map fst alocals) with (keys alocals) in *.
+  fwd eapply Forall2_nth_error_ex with (xs := keys alocals) as HH; eauto.
+    destruct HH as (ak & ? & ?).
+  fwd eapply Forall2_nth_error with (ys := blocals_ids); eauto. simpl in *.
+
+  repeat on >I_opt_value, invc.
+  eexists; split; eauto. constructor. congruence.
+
+- fwd eapply IHae; eauto.  break_exists. break_and.
+  on >I_value, invc.
+  fwd eapply Forall2_nth_error_ex with (xs := args) as HH; eauto.
+    destruct HH as (bv & ? & ?).
+
+  eexists; split; eauto. eapply B.eval_deref_constr; eauto.
+
+- fwd eapply IHae; eauto.  break_exists. break_and.
+  on >I_value, invc.
+  fwd eapply Forall2_nth_error_ex with (xs := free) as HH; eauto.
+    destruct HH as (bv & ? & ?).
+
+  eexists; split; eauto. eapply B.eval_deref_close; eauto.
+Qed.
+
+Lemma eval_sim_forall : forall M af aes avs bf bes,
+    I_frame M af bf ->
+    Forall2 (I_expr M) aes bes ->
+    Forall2 (A.eval af) aes avs ->
+    exists bvs,
+        B.eval_exprlist bf bes bvs /\
+        Forall2 (I_value M) avs bvs.
+first_induction aes; intros0 IIframe IIexpr Aeval;
+invc IIexpr; invc Aeval.
+- exists []. split; eauto. constructor.
+- fwd eapply eval_sim; eauto.  break_exists. break_and.
+  fwd eapply IHaes; eauto.  break_exists. break_and.
+  eexists. split; eauto. constructor; auto.
+Qed.
+
+Lemma nat_pos_nat : forall n,
+    pred (Pos.to_nat (Pos.of_succ_nat n)) = n.
+intros.  rewrite SuccNat2Pos.id_succ. reflexivity.
+Qed.
+
+Lemma I_env_nth_error : forall M AE BE afname af bfname,
+    I_env AE BE ->
+    nth_error AE afname = Some af ->
+    I_id M (IkFunc afname) bfname ->
+    exists bsym bf,
+        Genv.find_symbol BE bfname = Some bsym /\
+        Genv.find_funct_ptr BE bsym = Some bf /\
+        I_func M af bf.
+intros0 IIenv Afind IIid.
+Admitted.
+
+Inductive id_map_ok : id_map -> Prop :=
+| IdMapOk : forall M,
+        list_norepet (map snd M) ->
+        id_map_ok M.
+
+Lemma list_norepet_nth_error_unique' : forall A xs n (x : A),
+    nth_error xs n = Some x ->
+    list_norepet xs ->
+    ~ (exists n', n' <> n /\ nth_error xs n' = Some x).
+induction xs; intros0 Hnth Hnr.
+- destruct n; discriminate.
+- invc Hnr. destruct n; simpl in *.
+  + inject_some.
+    on (~ In _ _), contradict.
+    break_exists. break_and.  destruct x0; try congruence.
+    eapply nth_error_in. eauto.
+  + intro. break_exists. break_and.
+    destruct x0.
+    * simpl in *. inject_some.
+      on (~ In _ _), contradict.
+      eapply nth_error_in. eauto.
+    * simpl in *. eapply IHxs; eauto.
+      exists n. split; eauto.
+Qed.
+
+Lemma list_norepet_nth_error_unique : forall A xs n1 n2 (x : A),
+    nth_error xs n1 = Some x ->
+    nth_error xs n2 = Some x ->
+    list_norepet xs ->
+    n1 = n2.
+intros0 Hnth1 Hnth2 Hnr.
+destruct (eq_nat_dec n1 n2); eauto.
+exfalso. eapply list_norepet_nth_error_unique'; eauto.
+Qed.
+
+Lemma id_key_assoc_nth_error : forall V M k (v : V),
+    id_key_assoc M k = Some v ->
+    exists n, nth_error M n = Some (k, v).
+induction M; intros0 Hassoc; simpl in *.
+- discriminate.
+- destruct a. break_if.
+  + inject_some. exists 0. reflexivity.
+  + fwd eapply IHM as HH; eauto.  destruct HH as [n' ?].
+    exists (S n'). simpl. auto.
+Qed.
+
+Lemma I_id_ne : forall M k1 k2 i1 i2,
+    id_map_ok M ->
+    I_id M k1 i1 ->
+    I_id M k2 i2 ->
+    k1 <> k2 ->
+    i1 <> i2.
+intros0 Mok II1 II2 Hne.
+do 2 on >I_id, invc.
+unfold id_key_assoc in *.
+fwd eapply id_key_assoc_nth_error with (k := k1) as HH; eauto.
+  destruct HH as [n1 ?].
+fwd eapply id_key_assoc_nth_error with (k := k2) as HH; eauto.
+  destruct HH as [n2 ?].
+assert (HH : n1 <> n2) by congruence.
+contradict HH. eapply list_norepet_nth_error_unique.
+- eapply map_nth_error with (f := snd). eassumption.
+- change (snd (k1, i1)) with (snd (k2, i1)).
+  eapply map_nth_error. subst i1. assumption.
+- invc Mok. auto.
+Qed.
+
+Lemma zlookup_find_case : forall P tag (acases : list (Z * A.stmt)) acase bcases,
+    zlookup acases tag = Some acase ->
+    Forall2 (fun a b => fst a = fst b /\ P (snd a) (snd b)) acases bcases ->
+    exists bcase,
+        B.find_case tag bcases = Some bcase /\
+        P acase bcase.
+induction acases; intros0 Alook Hfa; invc Hfa; simpl in *.
+- discriminate.
+- destruct a as [ak acase']. destruct y as [bk bcase']. break_and. simpl in *.
+  unfold zeq. subst bk. break_if.
+  + inject_some. eauto.
+  + eapply IHacases; eauto.
+Qed.
+
+Theorem I_sim : forall M AE BE a a' b,
+    id_map_ok M ->
+    I_env AE BE ->
+    I M a b ->
+    A.sstep AE a a' ->
+    exists b',
+        B.step BE b E0 b' /\
+        I M a' b'.
+destruct a as [ae af ak | val ak | ae];
+intros0 Mok Henv II Astep; [ | | solve [invc Astep] ];
+inv Astep; inv II;
+try on >I_stmt, invc;
+simpl in *.
+
+- (* Seq *)
+  eexists. split. eapply B.step_seq; eauto.
+  i_ctor. i_ctor.
+
+- (* MkConstr *)
+  assert (be ! bdst = None) by admit.
+  fwd eapply eval_sim_forall as HH; eauto.  destruct HH as (bvs & ? & ?).
+  eexists. split. eapply B.step_make_constr; eauto.
+  i_ctor.
+
+- (* MkClose *)
+  assert (be ! bdst = None) by admit.
+  assert (fname < length AE) by admit.
+
+  rewrite <- nth_error_Some in *.
+  destruct (nth_error AE fname) eqn:?; try congruence.
+  fwd eapply I_env_nth_error as HH; eauto.
+    destruct HH as (bsym & bf & ? & ? & ?).
+
+  fwd eapply eval_sim_forall as HH; eauto.  destruct HH as (bvs & ? & ?).
+
+  eexists. split. eapply B.step_make_close; eauto.
+  i_ctor. i_lem set_I_frame. i_ctor. rewrite nat_pos_nat. auto.
+
+- (* MakeCall *)
+  assert (be ! bdst = None) by admit.
+
+  fwd eapply eval_sim with (ae := fe) as HH; eauto.  destruct HH as (bfe & ? & ?).
+  fwd eapply eval_sim with (ae := ae0) as HH; eauto.  destruct HH as (bae & ? & ?).
+  on (I_value _ (Close _ _) _), invc.
+
+  fwd eapply I_env_nth_error as HH; eauto.
+    destruct HH as (bsym & bfunc & ? & ? & ?).
+  on >I_func, inv.
+
+  eexists. split. eapply B.step_call; eauto. simpl.
+  i_ctor. 2: do 2 i_ctor.
+  i_ctor.
+  + rewrite PTree.gso, PTree.gss by (eapply I_id_ne; eauto; discriminate).
+    constructor. auto.
+  + rewrite PTree.gss. constructor. auto.
+
+- (* Switchinate *)
+  assert (be ! btargid = None) by admit.
+
+  fwd eapply eval_sim with (ae := A.Arg) as HH; eauto using A.EArg.
+    destruct HH as (btv & ? & ?).
+  on (A.arg af = _), fun H => rewrite H in *.
+  on >I_value, invc.
+
+  fwd eapply zlookup_find_case as HH; eauto.  destruct HH as (bcase & ? & ?).
+
+  eexists. split. eapply B.step_switch; eauto.
+  i_ctor. i_ctor.
+
+- (* Assign *)
+  assert (be ! bdst = None) by admit.
+
+  fwd eapply eval_sim as HH; eauto.  destruct HH as (bv & ? & ?).
+
+  eexists. split. eapply B.step_assign; eauto.
+  i_ctor.
+
+
+- (* ContSeq *)
+  on >I_cont, inv.
+
+  eexists. split. eapply B.step_skip_seq; eauto.
+  i_ctor.
+
+- (* ContSwitch *)
+  on >I_cont, inv.
+
+  eexists. split. eapply B.step_kswitch; eauto.
+  i_ctor.
+
+- (* ContReturn *)
+  on >I_cont, inv.
+  fwd eapply eval_sim as HH; eauto.  destruct HH as (bv & ? & ?).
+
+  eexists. split. eapply B.step_skip_return; eauto.
+  i_ctor.
+
+- (* ContStop *)
+  on >I_cont, inv.
+  admit.
+
+- (* ContCall *)
+  on >I_cont, inv.
+
+  eexists. split. eapply B.step_return; eauto.
+  i_ctor.
+
+Admitted.
+
+
 
 
 
 (* TODO *)
+
+
+
 
 
 
